Modularize timing automation and RISCV stuff, redid vtasksuspendall as a test

timing/.Makefile.d
@@ -1,12 +1,18 @@
-riscvTiming.vo riscvTiming.glob riscvTiming.v.beautified riscvTiming.required_vo: riscvTiming.v ../Picinae_core.vo ../Picinae_riscv.vo
-riscvTiming.vio: riscvTiming.v ../Picinae_core.vio ../Picinae_riscv.vio
-riscvTiming.vos riscvTiming.vok riscvTiming.required_vos: riscvTiming.v ../Picinae_core.vos ../Picinae_riscv.vos
-timing_auto.vo timing_auto.glob timing_auto.v.beautified timing_auto.required_vo: timing_auto.v riscvTiming.vo
-timing_auto.vio: timing_auto.v riscvTiming.vio
-timing_auto.vos timing_auto.vok timing_auto.required_vos: timing_auto.v riscvTiming.vos
-memsolve.vo memsolve.glob memsolve.v.beautified memsolve.required_vo: memsolve.v riscvTiming.vo
-memsolve.vio: memsolve.v riscvTiming.vio
-memsolve.vos memsolve.vok memsolve.required_vos: memsolve.v riscvTiming.vos
+TimingAutomation.vo TimingAutomation.glob TimingAutomation.v.beautified TimingAutomation.required_vo: TimingAutomation.v ../Picinae_core.vo ../Picinae_statics.vo ../Picinae_finterp.vo ../Picinae_theory.vo ../Picinae_simplifier_base.vo ../Picinae_simplifier_v1_1.vo
+TimingAutomation.vio: TimingAutomation.v ../Picinae_core.vio ../Picinae_statics.vio ../Picinae_finterp.vio ../Picinae_theory.vio ../Picinae_simplifier_base.vio ../Picinae_simplifier_v1_1.vio
+TimingAutomation.vos TimingAutomation.vok TimingAutomation.required_vos: TimingAutomation.v ../Picinae_core.vos ../Picinae_statics.vos ../Picinae_finterp.vos ../Picinae_theory.vos ../Picinae_simplifier_base.vos ../Picinae_simplifier_v1_1.vos
+riscv/CPUTimingBehavior.vo riscv/CPUTimingBehavior.glob riscv/CPUTimingBehavior.v.beautified riscv/CPUTimingBehavior.required_vo: riscv/CPUTimingBehavior.v 
+riscv/CPUTimingBehavior.vio: riscv/CPUTimingBehavior.v 
+riscv/CPUTimingBehavior.vos riscv/CPUTimingBehavior.vok riscv/CPUTimingBehavior.required_vos: riscv/CPUTimingBehavior.v 
+riscv/RISCVTiming.vo riscv/RISCVTiming.glob riscv/RISCVTiming.v.beautified riscv/RISCVTiming.required_vo: riscv/RISCVTiming.v ../Picinae_riscv.vo riscv/CPUTimingBehavior.vo TimingAutomation.vo
+riscv/RISCVTiming.vio: riscv/RISCVTiming.v ../Picinae_riscv.vio riscv/CPUTimingBehavior.vio TimingAutomation.vio
+riscv/RISCVTiming.vos riscv/RISCVTiming.vok riscv/RISCVTiming.required_vos: riscv/RISCVTiming.v ../Picinae_riscv.vos riscv/CPUTimingBehavior.vos TimingAutomation.vos
+riscv/NEORV32.vo riscv/NEORV32.glob riscv/NEORV32.v.beautified riscv/NEORV32.required_vo: riscv/NEORV32.v riscv/CPUTimingBehavior.vo
+riscv/NEORV32.vio: riscv/NEORV32.v riscv/CPUTimingBehavior.vio
+riscv/NEORV32.vos riscv/NEORV32.vok riscv/NEORV32.required_vos: riscv/NEORV32.v riscv/CPUTimingBehavior.vos
+memsolve.vo memsolve.glob memsolve.v.beautified memsolve.required_vo: memsolve.v riscv/RISCVTiming.vo
+memsolve.vio: memsolve.v riscv/RISCVTiming.vio
+memsolve.vos memsolve.vok memsolve.required_vos: memsolve.v riscv/RISCVTiming.vos
 examples/FreeRTOS/RTOSDemo_NoAsserts_Clz.vo examples/FreeRTOS/RTOSDemo_NoAsserts_Clz.glob examples/FreeRTOS/RTOSDemo_NoAsserts_Clz.v.beautified examples/FreeRTOS/RTOSDemo_NoAsserts_Clz.required_vo: examples/FreeRTOS/RTOSDemo_NoAsserts_Clz.v 
 examples/FreeRTOS/RTOSDemo_NoAsserts_Clz.vio: examples/FreeRTOS/RTOSDemo_NoAsserts_Clz.v 
 examples/FreeRTOS/RTOSDemo_NoAsserts_Clz.vos examples/FreeRTOS/RTOSDemo_NoAsserts_Clz.vok examples/FreeRTOS/RTOSDemo_NoAsserts_Clz.required_vos: examples/FreeRTOS/RTOSDemo_NoAsserts_Clz.v 
