timing/examples/FreeRTOS/tasks/eTaskGetState.v
@@ -1,0 +1,142 @@
+Require Import RTOSDemo_NoAsserts_Clz.
+Require Import riscvTiming.
+Import RISCVNotations.
+Require Import timing_auto.
+
+Module eTaskGetStateTime <: TimingModule.
+    Definition time_of_addr (s : store) (a : addr) : N :=
+        match neorv32_cycles_upper_bound s (RTOSDemo_NoAsserts_Clz a) with
+        | Some x => x | _ => 999 end.
+
+    Definition entry_addr : N := 0x80000958.
+
+    Definition exits (t:trace) : bool :=
+    match t with (Addr a,_)::_ => match a with
+    | 0x800009e8 | 0x800009f0 => true
+    | _ => false
+  end | _ => false end.
+End eTaskGetStateTime.
+
+Module eTaskGetStateAuto := TimingAutomation eTaskGetStateTime.
+Import eTaskGetStateTime eTaskGetStateAuto.
+
+Definition pxCurrentTCB (gp : N) (mem : addr -> N) : N :=
+    mem Ⓓ[gp ⊖ 1896].
+
+Definition time_of_eTaskGetState (mem : addr -> N) (gp a3 : N) (xTask : addr) (t : trace) :=
+  cycle_count_of_trace t =
+    time_mem + 2 +
+    if (pxCurrentTCB gp mem =? xTask) then (
+      time_branch + 2 + time_branch
+    ) else (
+      3 + 3 + 2 * time_mem + 2 + 3 * time_mem +
+      if (mem Ⓓ[0x80080004] =? 0) then (
+        3 + 3
+      ) else (
+        time_branch
+      ) +
+      2 + 2 +
+      if (xTask ⊕ 40 =? gp ⊖ 984) then (
+        time_branch + time_branch
+      ) else (
+        3 + 2 +
+        if (xTask ⊕ 20 =? mem Ⓓ[gp ⊖ 1900]) then (
+          time_branch + time_branch
+        ) else (
+          3 + if (xTask ⊕ 20 =? mem Ⓓ[gp ⊖ 1904]) then (
+            time_branch + time_branch
+          ) else (
+            3 + 2 + if (xTask ⊕ 20 =? gp ⊖ 1024) then (
+              3 + time_mem + 
+              if (xTask ⊕ 20 =? 0) then (
+                3 + time_mem + 2 +
+                if (99 =? xTask ⊕ 20) then (
+                    time_branch + time_branch
+                ) else (
+                    3 + time_mem + if (99 =? xTask ⊕ 20) then (
+                        time_branch + time_branch
+                    ) else (
+                        3 + time_mem + if (99 =? xTask ⊕ 20) then (
+                            time_branch + time_branch
+                        ) else (
+                            3 + 2 + time_branch
+                        )
+                    )
+                )
+              ) else (
+                time_branch + time_branch
+              )
+            ) else (
+              time_branch + 2 + 2 +
+              if (xTask ⊕ 20 =? gp ⊖ 1004) then (
+                time_branch + time_branch
+              ) else (
+                if (xTask ⊕ 20 =? 0) then (
+                  time_branch + time_branch
+                ) else (
+                  3 + 2 + time_branch
+                )
+              )
+            )
+          )
+        )
+      )
+    ).
+
+Definition eTaskGetState_timing_invs (s : store) (base_mem : addr -> N) (gp : N)
+    (a3 : N) (xTask : addr) (t:trace) : option Prop :=
+match t with (Addr a, s) :: t' => match a with
+| 0x80000958 => Some (s V_MEM32 = Ⓜbase_mem /\ s R_GP = Ⓓgp /\
+                        s R_A0 = ⒹxTask /\
+                        s R_A3 = Ⓓa3 /\
+                        cycle_count_of_trace t' = 0)
+| 0x800009e8 | 0x800009f0 => Some (time_of_eTaskGetState base_mem gp a3 xTask t)
+| _ => None end | _ => None end.
+
+Definition lifted_eTaskGetState : program :=
+    lift_riscv RTOSDemo_NoAsserts_Clz.
+
+(* We use simpl in a few convenient places: make sure it doesn't go haywire *)
+Arguments N.add _ _ : simpl nomatch.
+Arguments N.mul _ _ : simpl nomatch.
+
+Theorem eTaskGetState_timing:
+  forall s t s' x' base_mem gp a3 xTask
+         (ENTRY: startof t (x',s') = (Addr entry_addr, s))
+         (MDL: models rvtypctx s)
+         (MEM: s V_MEM32 = Ⓜbase_mem)
+         (GP: s R_GP = Ⓓgp)
+         (A0: s R_A0 = ⒹxTask)
+         (A3: s R_A3 = Ⓓa3),
+  satisfies_all 
+    lifted_eTaskGetState
+    (eTaskGetState_timing_invs s base_mem gp a3 xTask)
+    exits
+  ((x',s')::t).
+Proof using.
+    intros.
+    apply prove_invs.
+    Local Ltac step := time rv_step.
+
+    simpl. rewrite ENTRY. unfold entry_addr. step. auto.
+
+    intros.
+    eapply startof_prefix in ENTRY; try eassumption.
+    eapply preservation_exec_prog in MDL; 
+        try eassumption; [idtac|apply lift_riscv_welltyped].
+    clear - ENTRY PRE MDL. rename t1 into t. rename s1 into s'.
+
+    destruct_inv 32 PRE.
+    destruct PRE as (MEM & GP & A0 & A3 & Cycles).
+    repeat step.
+
+    { unfold time_of_eTaskGetState, pxCurrentTCB.
+        fold_big_subs. hammer. }
+
+    unfold time_of_eTaskGetState, pxCurrentTCB.
+        fold_big_subs. hammer.
+
+    par:
+        try solve [unfold time_of_eTaskGetState;
+        unfold pxCurrentTCB; fold_big_subs;
+        hammer].
