timing/riscv/RISCVTiming.v
@@ -1,0 +1,127 @@
+Require Export Picinae_riscv.
+Export RISCVNotations.
+Require Export CPUTimingBehavior.
+Require Export TimingAutomation.
+Require Export NArith.
+Require Import ZArith.
+Require Export Lia.
+Require Import List.
+Import ListNotations.
+
+Module Type ProgramInformation.
+    Parameter entry_addr : addr.
+    Parameter exits : trace -> bool.
+    (* Binary representation of the program to be decoded *)
+    Parameter binary : addr -> N.
+End ProgramInformation.
+
+Module RISCVTiming (cpu : CPUTimingBehavior) (prog : ProgramInformation) <: TimingModule IL_RISCV.
+    Export cpu prog.
+
+    Definition time_inf : N := 2^32.
+
+    Definition bop (s : store) (rs1 rs2 : N) (op : N -> N -> N) : N :=
+        let rs1var := if rs1 =? 0 then Ⓓ0 else s (rv_varid rs1) in
+        let rs2var := if rs2 =? 0 then Ⓓ0 else s (rv_varid rs2) in
+        match rs1var, rs2var with
+        | Ⓓr1, Ⓓr2 => op r1 r2
+        | _, _ => time_inf
+        end.
+
+    Definition cycles_per_instruction_at_addr (s : store) (a : addr) : N :=
+        match rv_decode (binary a) with
+        (* ==== I ISA Extension ==== *)
+        (* ALU *)
+        | R5_Add  _ _ _     => tadd
+        | R5_Addi _ _ _     => taddi
+        | R5_Slt  _ _ _     => tslt
+        | R5_Slti _ _ _     => tslti
+        | R5_Sltu _ _ _     => tsltu
+        | R5_Sltiu _ _ _    => tsltiu
+        | R5_Xor  _ _ _     => txor
+        | R5_Xori _ _ _     => txori
+        | R5_Or   _ _ _     => tor
+        | R5_Ori  _ _ _     => tori
+        | R5_And  _ _ _     => tand
+        | R5_Andi _ _ _     => tandi
+        | R5_Sub  _ _ _     => tsub
+        | R5_Lui  _ _       => tlui
+        | R5_Auipc _ _      => tauipc
+
+        (* ALU Shifts *)
+        | R5_Sll  _ _ shamt => tsll shamt
+        | R5_Slli _ _ shamt => tslli shamt
+        | R5_Srl  _ _ shamt => tsrl shamt
+        | R5_Srli _ _ shamt => tsrli shamt
+        | R5_Sra  _ _ shamt => tsra shamt
+        | R5_Srai _ _ shamt => tsrai shamt
+
+        (* Branches *)
+        | R5_Beq rs1 rs2 off => bop s rs1 rs2
+            (fun x y => if x =? y then ttbeq else tfbeq)
+        | R5_Bne rs1 rs2 off => bop s rs1 rs2
+            (fun x y => if negb (x =? y) then ttbeq else tfbeq)
+        | R5_Blt rs1 rs2 off => bop s rs1 rs2
+            (fun x y => if Z.ltb (toZ 32 x) (toZ 32 y) then ttbeq else tfbeq)
+        | R5_Bge rs1 rs2 off => bop s rs1 rs2
+            (fun x y => if Z.geb (toZ 32 x) (toZ 32 y) then ttbeq else tfbeq)
+        | R5_Bltu rs1 rs2 off => bop s rs1 rs2
+            (fun x y => if x <? y then ttbeq else tfbeq)
+        | R5_Bgeu rs1 rs2 off => bop s rs1 rs2
+            (fun x y => if negb (x <? y) then ttbeq else tfbeq)
+
+        (* Jump/call *)
+        | R5_Jal  _ _       => tjal
+        | R5_Jalr _ _ _     => tjalr
+
+        (* Load/store *)
+        | R5_Lb  _ _ _      => tlb
+        | R5_Lh  _ _ _      => tlh
+        | R5_Lw  _ _ _      => tlw
+        | R5_Lbu _ _ _      => tlbu
+        | R5_Lhu _ _ _      => tlhu
+        | R5_Sb  _ _ _      => tsb
+        | R5_Sh  _ _ _      => tsh
+        | R5_Sw  _ _ _      => tsw
+
+        (* Data fence *)
+        | R5_Fence   _ _    => tfence
+        | R5_Fence_i        => tfence
+
+        (* M extension *)
+
+        (* ==== M ISA Extension ==== *)
+        (* Multiplication *)
+        | R5_Mul    _ _ _   => tmul
+        | R5_Mulh   _ _ _   => tmulh
+        | R5_Mulsu  _ _ _   => tmulhsu
+        | R5_Mulu   _ _ _   => tmulhu
+
+        (* Division *)
+        | R5_Div    _ _ _   => tdiv
+        | R5_Divu   _ _ _   => tdivu
+        | R5_Rem    _ _ _   => trem
+        | R5_Remu   _ _ _   => tremu
+
+        (* ==== Zbb ISA Extension ==== *)
+        | R5_Clz r1 _       => tclz r1
+
+        | _ => time_inf
+        end.
+End RISCVTiming.
+
+Definition lift_riscv (f : addr -> N) (s : store) (a : addr) :=
+    Some (4, rv2il a (rv_decode (f a))).
+
+Theorem lift_riscv_welltyped:
+    forall p, welltyped_prog rvtypctx (lift_riscv p).
+Proof.
+    intros s a a0. unfold lift_riscv.
+    exists rvtypctx. apply welltyped_rv2il.
+Qed.
+
+(* Instantiate the Timing Automation module with RISC-V values *)
+(* Provide CPUTimingBehavior and ProgramInformation *)
+Module RISCVTimingAutomation := 
+    TimingAutomation IL_RISCV Statics_RISCV FInterp_RISCV 
+    PSimpl_RISCV_v1_1 Theory_RISCV.
